[WIP] Simplify lustretiming

theories/Languages/LustreTiming.v
@@ -3,6 +3,7 @@ From Reactive.Datatypes Require Ordered.
 From Reactive.Languages Require Lustre.
 
 From Stdlib Require Import Permutation.
+From Stdlib.Arith Require Import PeanoNat.
 
 Module Lustre := Lustre.
 
@@ -91,7 +92,7 @@ Definition freshness (seed: ident) (vars: list binder) := forall n, ~In (iter n 
 
 (* Translation from raw expressions to combinatorial expressions, extracting pre and arrow *)
 
-Fixpoint raw_to_comb {ty} (exp: raw_exp ty) (ident_origin: ident) (pre_binders: list binder) (pre_equations init_post_equations step_post_equations: list equation): (
+Fixpoint raw_to_comb {ty} (exp: raw_exp ty) (ident_origin: ident): (
     comb_exp ty (* init *)
     * comb_exp ty (* step *)
     * ident (* New identifier origin *)
@@ -109,18 +110,18 @@ Fixpoint raw_to_comb {ty} (exp: raw_exp ty) (ident_origin: ident) (pre_binders: 
     * (list equation) (* step_post equations *)
   ) :=
   match exp with
-    | Raw_EConst c => (EConst c, EConst c, ident_origin, pre_binders, pre_equations, init_post_equations, step_post_equations)
-    | Raw_EVar v => (EVar v, EVar v, ident_origin, pre_binders, pre_equations, init_post_equations, step_post_equations)
-    | Raw_EUnop u e => let '(ei, es, orig, binders, equations_pre, init_equations_post, step_equations_post) := raw_to_comb_aux e ident_origin pre_binders pre_equations init_post_equations step_post_equations in
-      (EUnop u ei, EUnop u es, orig, binders, equations_pre, init_equations_post, step_equations_post)
-    | Raw_EBinop b e1 e2 => let '(e1i, e1s, orig1, binders1, equations_pre1, init_equations_post1, step_equations_post1) := raw_to_comb_aux e1 ident_origin pre_binders pre_equations init_post_equations step_post_equations in
-      let '(e2i, e2s, orig2, binders2, equations_pre2, init_equations_post2, step_equations_post2) := raw_to_comb_aux e2 orig1 binders1 equations_pre1 init_equations_post1 step_equations_post1 in
-        (EBinop b e1i e2i, EBinop b e1s e2s, orig2, binders2, equations_pre2, init_equations_post2, step_equations_post2)
-    | Raw_EIfte e1 e2 e3 => let '(e1i, e1s, orig1, binders1, equations_pre1, init_equations_post1, step_equations_post1) := raw_to_comb_aux e1 ident_origin pre_binders pre_equations init_post_equations step_post_equations in
-      let '(e2i, e2s, orig2, binders2, equations_pre2, init_equations_post2, step_equations_post2) := raw_to_comb_aux e2 orig1 binders1 equations_pre1 init_equations_post1 step_equations_post1 in
-        let '(e3i, e3s, orig3, binders3, equations_pre3, init_equations_post3, step_equations_post3) := raw_to_comb_aux e3 orig2 binders2 equations_pre2 init_equations_post2 step_equations_post2 in
-        (EIfte e1i e2i e3i, EIfte e1s e2s e3s, orig3, binders3, equations_pre3, init_equations_post3, step_equations_post3)
-    | @Raw_EPre t e => let '(ei, es, ident_pre, binders, equations_pre, init_equations_post, step_equations_post) := raw_to_comb_aux e ident_origin pre_binders pre_equations init_post_equations step_post_equations in
+    | Raw_EConst c => (EConst c, EConst c, ident_origin, [], [], [], [])
+    | Raw_EVar v => (EVar v, EVar v, ident_origin, [], [], [], [])
+    | Raw_EUnop u e => let '(ei, es, orig, binders, eqs_pre, init_post, step_post) := raw_to_comb e ident_origin in
+      (EUnop u ei, EUnop u es, orig, binders, eqs_pre, init_post, step_post)
+    | Raw_EBinop b e1 e2 => let '(ei1, es1, orig1, binders1, eqs_pre1, init_post1, step_post1) := raw_to_comb e1 ident_origin in
+      let '(e2i, e2s, orig2, binders2, eqs_pre2, init_post2, step_post2) := raw_to_comb e2 orig1 in
+        (EBinop b ei1 e2i, EBinop b es1 e2s, orig2, binders1 ++ binders2, eqs_pre1 ++ eqs_pre2, init_post1 ++ init_post2, step_post1 ++ step_post2)
+    | Raw_EIfte e1 e2 e3 => let '(ei1, es1, orig1, binders1, eqs_pre1, init_post1, step_post1) := raw_to_comb e1 ident_origin in
+      let '(e2i, e2s, orig2, binders2, eqs_pre2, init_post2, step_post2) := raw_to_comb e2 orig1 in
+        let '(e3i, e3s, orig3, binders3, eqs_pre3, init_post3, step_post3) := raw_to_comb e3 orig2 in
+        (EIfte ei1 e2i e3i, EIfte es1 e2s e3s, orig3, binders1 ++ binders2 ++ binders3, eqs_pre1 ++ eqs_pre2 ++ eqs_pre3, init_post1 ++ init_post2 ++ init_post3, step_post1 ++ step_post2 ++ step_post3)
+    | @Raw_EPre t e => let '(ei, es, ident_pre, binders, eqs_pre, init_post, step_post) := raw_to_comb e ident_origin in
       let ident_eq := next_ident ident_pre in
         let next_orig := next_ident ident_eq in
           let pre_var := (ident_pre, t) in
@@ -130,103 +131,175 @@ Fixpoint raw_to_comb {ty} (exp: raw_exp ty) (ident_origin: ident) (pre_binders: 
                 EVar pre_var,
                 next_orig,
                 pre_var::eq_var::binders,
-                (ident_pre, existT comb_exp t (EVar eq_var))::equations_pre,
-                (ident_eq, existT _ t ei)::init_equations_post,
-                (ident_eq, existT _ t es)::step_equations_post
+                (ident_pre, existT comb_exp t (EVar eq_var))::eqs_pre,
+                (ident_eq, existT _ t ei)::init_post,
+                (ident_eq, existT _ t es)::step_post
               )
-    | Raw_EArrow e1 e2 => let '(e1i, e1s, orig1, binders1, equations_pre1, init_equations_post1, step_equations_post1) := raw_to_comb_aux e1 ident_origin pre_binders pre_equations init_post_equations step_post_equations in
-      let '(e2i, e2s, orig2, binders2, equations_pre2, init_equations_post2, step_equations_post2) := raw_to_comb_aux e2 orig1 binders1 equations_pre1 init_equations_post1 step_equations_post1 in
-        (e1i, e2s, orig2, binders2, equations_pre2, init_equations_post2, step_equations_post2)
+    | Raw_EArrow e1 e2 => let '(ei1, es1, orig1, binders1, eqs_pre1, init_post1, step_post1) := raw_to_comb e1 ident_origin in
+      let '(e2i, e2s, orig2, binders2, eqs_pre2, init_post2, step_post2) := raw_to_comb e2 orig1 in
+        (ei1, e2s, orig2, binders1 ++ binders2, eqs_pre1 ++ eqs_pre2, init_post1 ++ init_post2, step_post1 ++ step_post2)
   end.
 
-Definition raw_to_comb {ty} (exp: raw_exp ty) (ident_origin: ident): (
-    comb_exp ty (* init *)
-    * comb_exp ty (* step *)
-    * ident (* New identifier origin *)
-    * (list binder) (* Variables created for pre *)
-    * (list equation) (* pre equations *)
-    (* Equations to merge with the regular equations *)
-    (* for init: 
-      prex = undef (a variable initialised later)
-
-      for step:
-      prex = eqx (eqx being updated later with the current values)
-    *)
-    (* Equations NOT to be merged, but can be ordered separately *)
-    * (list equation) (* init_post equations *)
-    * (list equation) (* step_post equations *)
-  ) :=
-  raw_to_comb_aux exp ident_origin [] [] [] [].
-
 (** Properties *)
-
-Lemma freshness_raw_to_comb {ty} {exp: raw_exp ty} {ei es: comb_exp ty} {seed0 seed1: ident} {binders pre_binders0 pre_binders1: list binder} {pre_eqs0 pre_eqs1 init_post0 init_post1 step_post0 step_post1: list equation}:
-  raw_to_comb exp seed0 pre_binders0 pre_eqs0 init_post0 step_post0 = (ei, es, seed1, pre_binders1, pre_eqs1, init_post1, step_post1)
-  -> freshness seed0 (pre_binders0 ++ binders)
-  -> freshness seed1 (pre_binders1 ++ binders).
+Lemma freshness_fusion {seed: ident} {vars1 vars2: list binder}:
+  freshness seed vars1 -> freshness seed vars2 -> freshness seed (vars1 ++ vars2).
 Proof.
-  intros eqe isfresh.
-  induction exp in ei, es, seed0, seed1, pre_binders0, pre_binders1, pre_eqs0, pre_eqs1, init_post0, init_post1, step_post0, step_post1, eqe, isfresh.
-  - injection eqe as <- <- <- <- <- <- <-.
-    assumption.
-  - injection eqe as <- <- <- <- <- <- <-.
-    assumption.
-  - simpl in eqe.
-    destruct (raw_to_comb exp seed0 pre_binders0 pre_eqs0 init_post0 step_post0) as [[[[[[ei_1 es_1] seed_1] binders_1] pre_eqs_1] init_post_1] step_post_1] eqn: unfold1.
-    injection eqe as <- <- <- <- <- <- <-.
-    apply (IHexp _ _ _ _ _ _ _ _ _ _ _ _ unfold1 isfresh).
-  - simpl in eqe.
-    destruct (raw_to_comb exp1 seed0 pre_binders0 pre_eqs0 init_post0 step_post0) as [[[[[[ei_1 es_1] seed_1] binders_1] pre_eqs_1] init_post_1] step_post_1] eqn: unfold1.
-    destruct (raw_to_comb exp2 seed_1 binders_1 pre_eqs_1 init_post_1 step_post_1) as [[[[[[ei_2 es_2] seed_2] binders_2] pre_eqs_2] init_post_2] step_post_2] eqn: unfold2.
-    injection eqe as <- <- <- <- <- <- <-.
-    specialize (IHexp1 _ _ _ _ _ _ _ _ _ _ _ _ unfold1 isfresh).
-    specialize (IHexp2 _ _ _ _ _ _ _ _ _ _ _ _ unfold2 IHexp1).
-    assumption.
-  - simpl in eqe.
-    destruct (raw_to_comb exp1 seed0 pre_binders0 pre_eqs0 init_post0 step_post0) as [[[[[[ei_1 es_1] seed_1] binders_1] pre_eqs_1] init_post_1] step_post_1] eqn: unfold1.
-    destruct (raw_to_comb exp2 seed_1 binders_1 pre_eqs_1 init_post_1 step_post_1) as [[[[[[ei_2 es_2] seed_2] binders_2] pre_eqs_2] init_post_2] step_post_2] eqn: unfold2.
-    destruct (raw_to_comb exp3 seed_2 binders_2 pre_eqs_2 init_post_2 step_post_2) as [[[[[[ei_3 es_3] seed_3] binders_3] pre_eqs_3] init_post_3] step_post_3] eqn: unfold3.
-    injection eqe as <- <- <- <- <- <- <-.
-    specialize (IHexp1 _ _ _ _ _ _ _ _ _ _ _ _ unfold1 isfresh).
-    specialize (IHexp2 _ _ _ _ _ _ _ _ _ _ _ _ unfold2 IHexp1).
-    specialize (IHexp3 _ _ _ _ _ _ _ _ _ _ _ _ unfold3 IHexp2).
-    assumption.
-  - simpl in eqe.
-    destruct (raw_to_comb exp seed0 pre_binders0 pre_eqs0 init_post0 step_post0) as [[[[[[ei_1 es_1] seed_1] binders_1] pre_eqs_1] init_post_1] step_post_1] eqn: unfold1.
-    injection eqe as <- <- <- <- <- <- <-.
-    specialize (IHexp _ _ _ _ _ _ _ _ _ _ _ _ unfold1 isfresh).
-    intros n isin.
-    rewrite map_app in isin.
-    apply in_app_or in isin.
-    specialize (IHexp (S (S n))).
-    do 2 rewrite map_cons in isin.
-    unfold fst at 1 2 in isin.
-    rewrite map_app in IHexp.
-    rewrite in_app_iff in IHexp.
+  intros fresh1 fresh2 n.
+  specialize (fresh1 n).
+  specialize (fresh2 n).
+  rewrite map_app.
+  intro isin.
+  apply in_app_or in isin.
+  tauto.
+Qed.
 
-    rewrite <- !PeanoNat.Nat.iter_succ_r in isin.
-    destruct isin as [[is1 | [is2 | isin]] | isbinders].
-    + symmetry in is1.
-      apply ident_diff in is1.
-      assumption.
-    + symmetry in is2.
-      unfold next_ident at 2 in is2.
-      apply PeanoNat.Nat.succ_inj in is2.
-      apply ident_diff in is2.
-      assumption.
-    + apply IHexp.
-      left.
-      assumption.
-    + apply IHexp.
-      right.
-      assumption.
+Lemma freshness_later {seed1 seed2: ident} {n: nat} {vars: list binder}:
+  seed2 = iter n next_ident seed1 -> freshness seed1 vars -> freshness seed2 vars.
+Proof.
+  intros fresh1 isiter.
+  intro m.
+  specialize (isiter (m + n)).
+  rewrite Nat.iter_add in isiter.
+  rewrite <- fresh1 in isiter.
+  assumption.
+Qed.
+
+Lemma freshness_later_e {seed1 seed2: ident} {vars: list binder}:
+  (exists n, seed2 = iter n next_ident seed1) -> freshness seed1 vars -> freshness seed2 vars.
+Proof.
+  intros [n isiter].
+  apply (freshness_later isiter).
+Qed.
+
+Lemma raw_to_comb_nextseed {ty} {exp: raw_exp ty} {ei es: comb_exp ty} {seed seed': ident} {pre_binders: list binder} {pre_eqs init_post step_post: list equation}:
+  raw_to_comb exp seed = (ei, es, seed', pre_binders, pre_eqs, init_post, step_post)
+  -> exists n, seed' = iter n next_ident seed.
+Proof.
+  intro eqe.
+  induction exp in ei, es, seed, seed', pre_binders, pre_eqs, init_post, step_post, eqe.
+  - injection eqe as <- <- <- <- <- <- <-.
+    exists 0.
+    reflexivity.
+  - injection eqe as <- <- <- <- <- <- <-.
+    exists 0.
+    reflexivity.
   - simpl in eqe.
-    destruct (raw_to_comb exp1 seed0 pre_binders0 pre_eqs0 init_post0 step_post0) as [[[[[[ei_1 es_1] seed_1] binders_1] pre_eqs_1] init_post_1] step_post_1] eqn: unfold1.
-    destruct (raw_to_comb exp2 seed_1 binders_1 pre_eqs_1 init_post_1 step_post_1) as [[[[[[ei_2 es_2] seed_2] binders_2] pre_eqs_2] init_post_2] step_post_2] eqn: unfold2.
+    destruct (raw_to_comb exp seed) as [[[[[[ei1 es1] seed1] binders1] pre_eqs1] init_post1] step_post1] eqn: unfold1.
     injection eqe as <- <- <- <- <- <- <-.
-    specialize (IHexp1 _ _ _ _ _ _ _ _ _ _ _ _ unfold1 isfresh).
-    specialize (IHexp2 _ _ _ _ _ _ _ _ _ _ _ _ unfold2 IHexp1).
+    apply (IHexp _ _ _ _ _ _ _ _ unfold1).
+  - simpl in eqe.
+    destruct (raw_to_comb exp1 seed) as [[[[[[ei1 es1] seed1] binders1] pre_eqs1] init_post1] step_post1] eqn: unfold1.
+    destruct (raw_to_comb exp2 seed1) as [[[[[[ei2 es2] seed2] binders2] pre_eqs2] init_post2] step_post2] eqn: unfold2.
+    injection eqe as <- <- <- <- <- <- <-.
+    specialize (IHexp1 _ _ _ _ _ _ _ _ unfold1).
+    specialize (IHexp2 _ _ _ _ _ _ _ _ unfold2).
+    destruct IHexp1 as [n1 IHexp1].
+    destruct IHexp2 as [n2 IHexp2].
+    rewrite IHexp1 in IHexp2.
+    rewrite <- Nat.iter_add in IHexp2.
+    exists (n2 + n1).
+    assumption.
+  - simpl in eqe.
+    destruct (raw_to_comb exp1 seed) as [[[[[[ei1 es1] seed1] binders1] pre_eqs1] init_post1] step_post1] eqn: unfold1.
+    destruct (raw_to_comb exp2 seed1) as [[[[[[ei2 es2] seed2] binders2] pre_eqs2] init_post2] step_post2] eqn: unfold2.
+    destruct (raw_to_comb exp3 seed2) as [[[[[[ei3 es3] seed3] binders3] pre_eqs3] init_post3] step_post3] eqn: unfold3.
+    injection eqe as <- <- <- <- <- <- <-.
+    specialize (IHexp1 _ _ _ _ _ _ _ _ unfold1).
+    specialize (IHexp2 _ _ _ _ _ _ _ _ unfold2).
+    specialize (IHexp3 _ _ _ _ _ _ _ _ unfold3).
+    destruct IHexp1 as [n1 IHexp1].
+    destruct IHexp2 as [n2 IHexp2].
+    destruct IHexp3 as [n3 IHexp3].
+    rewrite IHexp1 in IHexp2.
+    rewrite IHexp2 in IHexp3.
+    do 2 rewrite <- Nat.iter_add in IHexp3.
+    exists (n3 + n2 + n1).
+    assumption.
+  - simpl in eqe.
+    destruct (raw_to_comb exp seed) as [[[[[[ei1 es1] seed1] binders1] pre_eqs1] init_post1] step_post1] eqn: unfold1.
+    injection eqe as <- <- <- <- <- <- <-.
+    specialize (IHexp _ _ _ _ _ _ _ _ unfold1).
+    destruct IHexp as [n IHexp].
+    exists (S (S n)).
+    simpl.
+    do 2 f_equal.
+    assumption.
+  - simpl in eqe.
+    destruct (raw_to_comb exp1 seed) as [[[[[[ei1 es1] seed1] binders1] pre_eqs1] init_post1] step_post1] eqn: unfold1.
+    destruct (raw_to_comb exp2 seed1) as [[[[[[ei2 es2] seed2] binders2] pre_eqs2] init_post2] step_post2] eqn: unfold2.
+    injection eqe as <- <- <- <- <- <- <-.
+    specialize (IHexp1 _ _ _ _ _ _ _ _ unfold1).
+    specialize (IHexp2 _ _ _ _ _ _ _ _ unfold2).
+    destruct IHexp1 as [n1 IHexp1].
+    destruct IHexp2 as [n2 IHexp2].
+    rewrite IHexp1 in IHexp2.
+    rewrite <- Nat.iter_add in IHexp2.
+    exists (n2 + n1).
+    assumption.
+Qed.
+
+Lemma freshness_raw_to_comb {ty} {exp: raw_exp ty} {ei es: comb_exp ty} {seed seed': ident} {pre_binders: list binder} {pre_eqs init_post step_post: list equation}:
+  raw_to_comb exp seed = (ei, es, seed', pre_binders, pre_eqs, init_post, step_post)
+  -> freshness seed' pre_binders.
+Proof.
+  intros eqe.
+  induction exp in ei, es, seed, seed', pre_binders, pre_eqs, init_post, step_post, eqe.
+  - injection eqe as <- <- <- <- <- <- <-.
+    intro n.
+    tauto.
+  - injection eqe as <- <- <- <- <- <- <-.
+    intro n.
+    tauto.
+  - simpl in eqe.
+    destruct (raw_to_comb exp seed) as [[[[[[ei1 es1] seed1] binders1] pre_eqs1] init_post1] step_post1] eqn: unfold1.
+    injection eqe as <- <- <- <- <- <- <-.
+    apply (IHexp _ _ _ _ _ _ _ _ unfold1).
+  - simpl in eqe.
+    destruct (raw_to_comb exp1 seed) as [[[[[[ei1 es1] seed1] binders1] pre_eqs1] init_post1] step_post1] eqn: unfold1.
+    destruct (raw_to_comb exp2 seed1) as [[[[[[ei2 es2] seed2] binders2] pre_eqs2] init_post2] step_post2] eqn: unfold2.
+    injection eqe as <- <- <- <- <- <- <-.
+    specialize (IHexp1 _ _ _ _ _ _ _ _ unfold1).
+    specialize (IHexp2 _ _ _ _ _ _ _ _ unfold2).
+    assert (nextseed := raw_to_comb_nextseed unfold2).
+    apply (freshness_later_e nextseed) in IHexp1.
+    apply (freshness_fusion IHexp1 IHexp2).
+  - simpl in eqe.
+    destruct (raw_to_comb exp1 seed) as [[[[[[ei1 es1] seed1] binders1] pre_eqs1] init_post1] step_post1] eqn: unfold1.
+    destruct (raw_to_comb exp2 seed1) as [[[[[[ei2 es2] seed2] binders2] pre_eqs2] init_post2] step_post2] eqn: unfold2.
+    destruct (raw_to_comb exp3 seed2) as [[[[[[ei3 es3] seed3] binders3] pre_eqs3] init_post3] step_post3] eqn: unfold3.
+    injection eqe as <- <- <- <- <- <- <-.
+    specialize (IHexp1 _ _ _ _ _ _ _ _ unfold1).
+    specialize (IHexp2 _ _ _ _ _ _ _ _ unfold2).
+    specialize (IHexp3 _ _ _ _ _ _ _ _ unfold3).
+    assert (nextseed1 := raw_to_comb_nextseed unfold2).
+    assert (nextseed2 := raw_to_comb_nextseed unfold3).
+    apply (freshness_later_e nextseed1) in IHexp1.
+    apply (freshness_later_e nextseed2) in IHexp1.
+    apply (freshness_later_e nextseed2) in IHexp2.
+    apply (freshness_fusion IHexp1 (freshness_fusion IHexp2 IHexp3)).
+  - simpl in eqe.
+    destruct (raw_to_comb exp) as [[[[[[ei1 es1] seed1] binders1] pre_eqs1] init_post1] step_post1] eqn: unfold1.
+    injection eqe as <- <- <- <- <- <- <-.
+    specialize (IHexp _ _ _ _ _ _ _ _ unfold1).
     intros n isin.
-    specialize (IHexp2 n).
-    contradiction.
+    rewrite <- !PeanoNat.Nat.iter_succ_r in isin.
+    rewrite !map_cons in isin.
+    unfold fst at 1 2 in isin.
+    destruct isin as [f | [f | isin]].
+    + apply ident_diff in f.
+      assumption.
+    + rewrite Nat.iter_succ_r in f.
+      apply ident_diff in f.
+      assumption.
+    + specialize (IHexp (S (S n))).
+      contradiction.
+  - simpl in eqe.
+    destruct (raw_to_comb exp1 seed) as [[[[[[ei1 es1] seed1] binders1] pre_eqs1] init_post1] step_post1] eqn: unfold1.
+    destruct (raw_to_comb exp2 seed1) as [[[[[[ei2 es2] seed2] binders2] pre_eqs2] init_post2] step_post2] eqn: unfold2.
+    injection eqe as <- <- <- <- <- <- <-.
+    specialize (IHexp1 _ _ _ _ _ _ _ _ unfold1).
+    specialize (IHexp2 _ _ _ _ _ _ _ _ unfold2).
+    assert (nextseed := raw_to_comb_nextseed unfold2).
+    apply (freshness_later_e nextseed) in IHexp1.
+    apply (freshness_fusion IHexp1 IHexp2).
 Qed.
